refactored typing

thys/First_Order_Clause/Ground_Typing.thy
@@ -5,9 +5,6 @@ theory Ground_Typing
     Term_Typing
 begin
 
-inductive typed for \<F> where
-  GFun: "\<F> f (length ts) = (\<tau>s, \<tau>) \<Longrightarrow> typed \<F> (GFun f ts) \<tau>"
-
 inductive welltyped for \<F> where
   GFun: "\<F> f (length ts) = (\<tau>s, \<tau>) \<Longrightarrow> list_all2 (welltyped \<F>) ts \<tau>s \<Longrightarrow> welltyped \<F> (GFun f ts) \<tau>"
 
@@ -15,23 +12,10 @@ locale ground_term_typing =
   fixes \<F> :: "('f, 'ty) fun_types"
 begin
 
-abbreviation typed where "typed \<equiv> Ground_Typing.typed \<F>"
 abbreviation welltyped where "welltyped \<equiv> Ground_Typing.welltyped \<F>"
 
-sublocale base_typing where typed = typed and welltyped = welltyped
+sublocale typing where welltyped = welltyped
 proof unfold_locales
-
-  show "right_unique typed"
-  proof (rule right_uniqueI)
-    fix t \<tau>\<^sub>1 \<tau>\<^sub>2
-
-    assume "typed t \<tau>\<^sub>1" and "typed t \<tau>\<^sub>2"
-
-    thus "\<tau>\<^sub>1 = \<tau>\<^sub>2"
-      by (auto elim!: typed.cases)
-  qed
-next
-
   show "right_unique welltyped"
   proof (rule right_uniqueI)
     fix t \<tau>\<^sub>1 \<tau>\<^sub>2
@@ -41,16 +25,10 @@ next
     thus "\<tau>\<^sub>1 = \<tau>\<^sub>2"
       by (auto elim!: welltyped.cases)
   qed
-next
-  fix t \<tau>
-
-  assume "welltyped t \<tau>"
-
-  then show "typed t \<tau>"
-    by (metis typed.intros welltyped.cases)
 qed
 
-sublocale term_typing where typed = typed and welltyped = welltyped and Fun = GFun
+sublocale term_typing where
+  welltyped = welltyped and Fun = GFun
 proof unfold_locales
   fix t t' c \<tau> \<tau>'
 
@@ -96,24 +74,12 @@ proof unfold_locales
       by simp
   qed
 next
-  fix t t' c \<tau> \<tau>'
-
-  assume "typed t \<tau>'" "typed t' \<tau>'" "typed c\<langle>t\<rangle>\<^sub>G \<tau>"
-
-  then show "typed c\<langle>t'\<rangle>\<^sub>G \<tau>"
-    by(induction c arbitrary: \<tau>) (auto simp: typed.simps)
-next
   fix f ts \<tau>
 
   assume "welltyped (GFun f ts) \<tau>"
 
   then show "\<forall>t\<in>set ts. \<exists>\<tau>'. welltyped t \<tau>'"
     by (metis gterm.inject in_set_conv_nth list_all2_conv_all_nth welltyped.simps)
-next
-  fix t
-
-  show "is_typed t"
-    by (cases t) (simp add: split_pairs2 typed.simps)
 qed
 
 end
@@ -121,9 +87,10 @@ end
 locale ground_typing = "term": ground_term_typing
 begin
 
-sublocale clause_typing where term_typed = term.typed and term_welltyped = term.welltyped
+sublocale clause_typing where term_welltyped = term.welltyped
   by unfold_locales
 
 end
+
 
 end
