thys/First_Order_Clause/Nonground_Typing.thy
@@ -15,31 +15,23 @@ locale nonground_typed_lifting =
   typed_grounding_functional_substitution_lifting
 
 locale nonground_typing_lifting =
-  is_typed: nonground_typed_lifting +
   is_welltyped: nonground_typed_lifting where
-  sub_typed = sub_welltyped and base_typed = base_welltyped 
-for base_welltyped sub_welltyped
+    sub_welltyped = sub_welltyped and base_welltyped = base_welltyped 
+  for base_welltyped sub_welltyped
 begin
 
-abbreviation "is_typed_ground_instance \<equiv> is_typed.is_typed_ground_instance"
+abbreviation "is_welltyped_ground_instance \<equiv> is_welltyped.is_welltyped_ground_instance"
 
-abbreviation "is_welltyped_ground_instance \<equiv> is_welltyped.is_typed_ground_instance"
+abbreviation "welltyped_ground_instances \<equiv> is_welltyped.welltyped_ground_instances"
 
-abbreviation "typed_ground_instances \<equiv> is_typed.typed_ground_instances"
-
-abbreviation "welltyped_ground_instances \<equiv> is_welltyped.typed_ground_instances"
-
-lemmas typed_ground_instances_def = is_typed.typed_ground_instances_def
-
-lemmas welltyped_ground_instances_def = is_welltyped.typed_ground_instances_def
+lemmas welltyped_ground_instances_def = is_welltyped.welltyped_ground_instances_def
 
 end
 
 locale nonground_inhabited_typing_lifting =
   nonground_typing_lifting +
-  typed: inhabited_typed_functional_substitution_lifting where base_typed = base_typed +
   welltyped: inhabited_typed_functional_substitution_lifting where
-  sub_typed = sub_welltyped and base_typed = base_welltyped
+  sub_welltyped = sub_welltyped and base_welltyped = base_welltyped
 
 locale term_based_nonground_typing_lifting =
   "term": nonground_term +
@@ -57,30 +49,28 @@ locale nonground_typing =
   for \<F> :: "('f, 'ty) fun_types"
 begin
 
-sublocale clause_typing "typed (\<V> :: ('v, 'ty) var_types)" "welltyped \<V>"
+sublocale clause_typing "welltyped \<V>"
   by unfold_locales
 
 sublocale atom: term_based_nonground_typing_lifting where
-  base_typed = typed and base_welltyped = welltyped and map = map_uprod and to_set = set_uprod and 
-  sub_typed = typed and sub_welltyped = welltyped and sub_to_ground = term.to_ground and
+  base_welltyped = welltyped and map = map_uprod and to_set = set_uprod and 
+  sub_welltyped = welltyped and sub_to_ground = term.to_ground and
   sub_from_ground = term.from_ground and to_ground_map = map_uprod and
   from_ground_map = map_uprod and ground_map = map_uprod and to_set_ground = set_uprod and
   sub_subst = "(\<cdot>t)" and sub_vars = term.vars
   by unfold_locales
 
 sublocale literal: term_based_nonground_typing_lifting where
-  base_typed = typed and
   base_welltyped = welltyped and sub_vars = atom.vars and sub_subst = "(\<cdot>a)" and
-  map = map_literal and to_set = set_literal and sub_typed = atom.typed and
-  sub_welltyped = atom.welltyped and sub_to_ground = atom.to_ground and
-  sub_from_ground = atom.from_ground and to_ground_map = map_literal and
-  from_ground_map = map_literal and ground_map = map_literal and to_set_ground = set_literal
+  map = map_literal and to_set = set_literal and sub_welltyped = atom.welltyped and
+  sub_to_ground = atom.to_ground and sub_from_ground = atom.from_ground and
+  to_ground_map = map_literal and from_ground_map = map_literal and ground_map = map_literal and
+  to_set_ground = set_literal
   by unfold_locales
 
 sublocale clause: term_based_nonground_typing_lifting where
-  base_typed = typed and base_welltyped = welltyped and
-  sub_vars = literal.vars and sub_subst = "(\<cdot>l)" and map = image_mset and to_set = set_mset and
-  sub_typed = literal.typed and sub_welltyped = literal.welltyped and
+  base_welltyped = welltyped and sub_vars = literal.vars and sub_subst = "(\<cdot>l)" and
+  map = image_mset and to_set = set_mset and sub_welltyped = literal.welltyped and
   sub_to_ground = literal.to_ground and sub_from_ground = literal.from_ground and
   to_ground_map = image_mset and from_ground_map = image_mset and ground_map = image_mset and
   to_set_ground = set_mset
@@ -95,25 +85,25 @@ locale nonground_inhabited_typing =
 begin
 
 sublocale atom: term_based_nonground_inhabited_typing_lifting where
-  base_typed = typed and base_welltyped = welltyped and map = map_uprod and to_set = set_uprod and 
-  sub_typed = typed and sub_welltyped = welltyped and sub_to_ground = term.to_ground and
+  base_welltyped = welltyped and map = map_uprod and to_set = set_uprod and 
+  sub_welltyped = welltyped and sub_to_ground = term.to_ground and
   sub_from_ground = term.from_ground and to_ground_map = map_uprod and 
   from_ground_map = map_uprod and ground_map = map_uprod and to_set_ground = set_uprod and 
   sub_subst = "(\<cdot>t)" and sub_vars = term.vars
   by unfold_locales
 
 sublocale literal: term_based_nonground_inhabited_typing_lifting where
-  base_typed = typed and base_welltyped = welltyped and sub_vars = atom.vars and 
-  sub_subst = "(\<cdot>a)" and map = map_literal and to_set = set_literal and sub_typed = atom.typed and
+  base_welltyped = welltyped and sub_vars = atom.vars and 
+  sub_subst = "(\<cdot>a)" and map = map_literal and to_set = set_literal and
   sub_welltyped = atom.welltyped and sub_to_ground = atom.to_ground and
   sub_from_ground = atom.from_ground and to_ground_map = map_literal and
   from_ground_map = map_literal and ground_map = map_literal and to_set_ground = set_literal
   by unfold_locales
 
 sublocale clause: term_based_nonground_inhabited_typing_lifting where
-  base_typed = typed and base_welltyped = welltyped and
+  base_welltyped = welltyped and
   sub_vars = literal.vars and sub_subst = "(\<cdot>l)" and map = image_mset and to_set = set_mset and
-  sub_typed = literal.typed and sub_welltyped = literal.welltyped and
+  sub_welltyped = literal.welltyped and
   sub_to_ground = literal.to_ground and sub_from_ground = literal.from_ground and
   to_ground_map = image_mset and from_ground_map = image_mset and ground_map = image_mset and
   to_set_ground = set_mset
