thys/First_Order_Clause/Typed_Functional_Substitution_Example.thy
@@ -6,27 +6,15 @@ begin
 
 type_synonym ('f, 'ty) fun_types = "'f \<Rightarrow> 'ty list \<times> 'ty"
 
-text \<open>Inductive predicates defining well-typed terms.\<close>
-inductive typed :: "('f, 'ty) fun_types \<Rightarrow> ('v, 'ty) var_types \<Rightarrow> ('f,'v) term \<Rightarrow> 'ty \<Rightarrow> bool"
-  for \<F> \<V> where
-    Var: "\<V> x = \<tau> \<Longrightarrow> typed \<F> \<V> (Var x) \<tau>"
-  | Fun: "\<F> f = (\<tau>s, \<tau>) \<Longrightarrow> typed \<F> \<V> (Fun f ts) \<tau>"
+text \<open>Inductive predicate defining well-typed terms.\<close>
 
 inductive welltyped :: "('f, 'ty) fun_types \<Rightarrow> ('v, 'ty) var_types \<Rightarrow> ('f,'v) term \<Rightarrow> 'ty \<Rightarrow> bool"
   for \<F> \<V> where
     Var: "\<V> x = \<tau> \<Longrightarrow> welltyped \<F> \<V> (Var x) \<tau>"
   | Fun: "\<F> f = (\<tau>s, \<tau>) \<Longrightarrow> list_all2 (welltyped \<F> \<V>) ts \<tau>s \<Longrightarrow> welltyped \<F> \<V> (Fun f ts) \<tau>"
 
-global_interpretation "term": base_typing "typed \<F> \<V>" "welltyped \<F> \<V>"
+global_interpretation "term": base_typing "welltyped \<F> \<V>"
 proof unfold_locales
-  show "right_unique (typed \<F> \<V>)"
-  proof (rule right_uniqueI)
-    fix t \<tau>\<^sub>1 \<tau>\<^sub>2
-    assume "typed \<F> \<V> t \<tau>\<^sub>1" and "typed \<F> \<V> t \<tau>\<^sub>2"
-    thus "\<tau>\<^sub>1 = \<tau>\<^sub>2"
-      by (auto elim!: typed.cases)
-  qed
-next
   show "right_unique (welltyped \<F> \<V>)"
   proof (rule right_uniqueI)
     fix t \<tau>\<^sub>1 \<tau>\<^sub>2
@@ -34,46 +22,25 @@ next
     thus "\<tau>\<^sub>1 = \<tau>\<^sub>2"
       by (auto elim!: welltyped.cases)
   qed
-next
-  fix t \<tau>
-  assume "welltyped \<F> \<V> t \<tau>"
-  then show "typed \<F> \<V> t \<tau>"
-    by (metis (full_types) typed.simps welltyped.cases)
 qed
 
 global_interpretation functional_substitution_typing where
-  typed = "typed (\<F> :: ('f, 'ty) fun_types)" and welltyped = "welltyped \<F>" and
+  welltyped = "welltyped \<F>" and
   subst = subst_apply_term and id_subst = Var and comp_subst = subst_compose and
   vars = "vars_term :: ('f, 'v) term \<Rightarrow> 'v set"
-  by unfold_locales (simp_all add: typed.Var  welltyped.Var)
+  for \<F> :: "('f, 'ty) fun_types"
+  by unfold_locales (simp_all add: welltyped.Var)
 
 text \<open>A selection of substitution properties for typed terms.\<close>
 locale typed_term_subst_properties =
-  typed: base_typed_subst_stability where typed = "typed \<F>" +
-  welltyped: base_typed_subst_stability where typed = "welltyped \<F>"
-for \<F> :: "('f, 'ty) fun_types"
+  welltyped: base_typed_subst_stability where welltyped = "welltyped \<F>"
+  for \<F> :: "('f, 'ty) fun_types"
 
 global_interpretation "term": typed_term_subst_properties where
   subst = subst_apply_term and id_subst = Var and comp_subst = subst_compose and
   vars = "vars_term :: ('f, 'v) term \<Rightarrow> 'v set" and \<F> = \<F>
-for \<F> :: "'f \<Rightarrow> 'ty list \<times> 'ty"
+  for \<F> :: "'f \<Rightarrow> 'ty list \<times> 'ty"
 proof (unfold_locales)
-  fix \<tau> and \<V> and t :: "('f, 'v) term" and \<sigma>
-  assume is_typed_on: "\<forall>x \<in> vars_term t. typed \<F> \<V> (\<sigma> x) (\<V> x)"
-
-  show "typed \<F> \<V> (t \<cdot> \<sigma>) \<tau> \<longleftrightarrow> typed \<F> \<V> t \<tau>"
-  proof(rule iffI)
-    assume "typed \<F> \<V> t \<tau>"
-    then show "typed \<F> \<V> (t \<cdot> \<sigma>) \<tau>"
-      using is_typed_on
-      by(induction rule: typed.induct)(auto simp: typed.Fun)
-  next
-    assume "typed \<F> \<V> (t \<cdot> \<sigma>) \<tau>"
-    then show "typed \<F> \<V> t \<tau>"
-      using is_typed_on
-      by(induction t)(auto simp: typed.simps)
-  qed
-next
   fix \<V> :: "('v, 'ty) var_types" and t :: "('f, 'v) term" and \<sigma> \<tau>
   assume is_welltyped_on: "\<forall>x \<in> vars_term t. welltyped \<F> \<V> (\<sigma> x) (\<V> x)"
 
@@ -119,26 +86,20 @@ next
   qed
 qed
 
+find_theorems name: "is_welltyped_subst_update"
+
 text \<open>Examples of generated lemmas and definitions\<close>
 thm
-  term.welltyped.right_unique
+  (* term.welltyped.right_unique *)
+  term.right_unique                        
   term.welltyped.subst_stability
 
-  term.typed.right_unique
-  term.typed.subst_stability
-
   is_welltyped_subst_update
-  is_typed_subst_update
   is_welltyped_on_subset
-  is_typed_on_subset
   is_welltyped_id_subst
-  is_typed_id_subst
 
 term term.is_welltyped
 term is_welltyped_on
 term is_welltyped
-term term.is_typed
-term is_typed_on
-term is_typed
 
 end
