thys/First_Order_Clause/Typing.thy
@@ -2,104 +2,48 @@ theory Typing
   imports Main
 begin
 
-locale typed =
-  fixes typed :: "'expr \<Rightarrow> 'ty \<Rightarrow> bool"
-  assumes right_unique: "right_unique typed"
+locale typing =
+  fixes welltyped :: "'expr \<Rightarrow> 'ty \<Rightarrow> bool"
+  assumes right_unique: "right_unique welltyped"
 begin
 
 lemmas right_uniqueD [dest] = right_uniqueD[OF right_unique]
 
 end
 
-locale base_typed = typed
+locale base_typing = typing
 begin
 
-abbreviation is_typed where 
-  "is_typed expr \<equiv> \<exists>\<tau>. typed expr \<tau>"
+abbreviation is_welltyped where 
+  "is_welltyped expr \<equiv> \<exists>\<tau>. welltyped expr \<tau>"
 
 end
 
-(* TODO: Generalize? *)
-locale typed_lifting =
-  sub: typed where typed = sub_typed 
-for sub_typed :: "'sub \<Rightarrow> 'ty \<Rightarrow> bool" +
-fixes to_set :: "'expr \<Rightarrow> 'sub set" 
+locale typing_lifting = sub: typing where welltyped = sub_welltyped 
+  for sub_welltyped :: "'sub \<Rightarrow> 'ty \<Rightarrow> bool" +
+  fixes to_set :: "'expr \<Rightarrow> 'sub set" 
 begin
 
-definition is_typed where
-  "is_typed expr \<equiv> \<exists>\<tau>. \<forall>sub \<in> to_set expr. sub_typed sub \<tau>"
+definition is_welltyped where
+  "is_welltyped expr \<equiv> \<exists>\<tau>. \<forall>sub \<in> to_set expr. sub_welltyped sub \<tau>"
 
-abbreviation typed where
-  "typed expr (_::unit) \<equiv> is_typed expr"
+abbreviation welltyped where
+  "welltyped expr (_::unit) \<equiv> is_welltyped expr"
 
-sublocale typed where typed = typed
+sublocale typing where welltyped = welltyped
   by unfold_locales (auto simp: right_unique_def)
 
 end
 
-locale typing =
-  typed: typed where typed = typed +
-  welltyped: typed where typed = welltyped
-for typed welltyped :: "'expr \<Rightarrow> 'ty \<Rightarrow> bool" +
-assumes typed_if_welltyped: "\<And>expr \<tau>. welltyped expr \<tau> \<Longrightarrow> typed expr \<tau>"
-
-locale base_typing =
-  typing +
-  typed: base_typed where typed = typed +
-  welltyped: base_typed where typed = welltyped
-begin
-
-abbreviation is_typed where
-  "is_typed \<equiv> typed.is_typed"
-
-abbreviation is_welltyped where
-  "is_welltyped \<equiv> welltyped.is_typed"
-
-lemma is_typed_if_is_welltyped: "is_welltyped expr \<Longrightarrow> is_typed expr"
-  using typed_if_welltyped
-  by blast
-
-end
-
-locale typing_lifting = 
- sub: typing where typed = sub_typed and welltyped = sub_welltyped +
- typed: typed_lifting where sub_typed = sub_typed +
- welltyped: typed_lifting where sub_typed = sub_welltyped
-for sub_typed sub_welltyped :: "'sub \<Rightarrow> 'ty \<Rightarrow> bool"
-begin
-
-abbreviation typed where
-  "typed \<equiv> typed.typed"
-
-abbreviation welltyped where
-  "welltyped \<equiv> welltyped.typed"
-
-abbreviation is_typed where
-  "is_typed \<equiv> typed.is_typed"
-
-abbreviation is_welltyped where
-  "is_welltyped \<equiv> welltyped.is_typed"
-
-lemmas is_typed_def = typed.is_typed_def
-
-lemmas is_welltyped_def = welltyped.is_typed_def
-
-sublocale typing where typed = typed and welltyped = welltyped
-  by unfold_locales (auto simp: is_typed_def is_welltyped_def intro: sub.typed_if_welltyped)
-
-lemmas is_typed_if_is_welltyped = typed_if_welltyped
-
-end
-
 locale typing_lifting' =
-fixes
-  sub_typed sub_welltyped :: "'extra \<Rightarrow> 'sub \<Rightarrow> 'ty' \<Rightarrow> bool" and 
-  to_set :: "'expr \<Rightarrow> 'sub set"
-assumes lifting: "\<And>extra. typing_lifting (sub_typed extra) (sub_welltyped extra)"
+  fixes
+    sub_welltyped :: "'extra \<Rightarrow> 'sub \<Rightarrow> 'ty' \<Rightarrow> bool" and 
+    to_set :: "'expr \<Rightarrow> 'sub set"
+  assumes lifting: "\<And>extra. typing_lifting (sub_welltyped extra)"
 begin
 
 sublocale typing_lifting where
-  sub_typed = "sub_typed \<V>" and sub_welltyped = "sub_welltyped \<V>" and to_set = to_set
+  sub_welltyped = "sub_welltyped \<V>" and to_set = to_set
   by (rule lifting)
 
 end
