thys/First_Order_Clause/Clause_Typing.thy
@@ -7,19 +7,13 @@ theory Clause_Typing
     Uprod_Extra
 begin
 
-locale clause_typing =
-  "term": typing term_typed term_welltyped
-  for term_typed term_welltyped
+locale clause_typing = "term": typing term_welltyped
+  for term_welltyped
 begin
 
 sublocale atom: typing_lifting where
-  sub_typed = term_typed and sub_welltyped = term_welltyped and to_set = set_uprod
+  sub_welltyped = term_welltyped and to_set = set_uprod
   by unfold_locales
-
-lemma atom_is_typed_iff [simp]:
-  "atom.is_typed (Upair t t') \<longleftrightarrow> (\<exists>\<tau>. term_typed t \<tau> \<and> term_typed t' \<tau>)"
-  unfolding atom.is_typed_def
-  by simp
 
 lemma atom_is_welltyped_iff [simp]:
   "atom.is_welltyped (Upair t t') \<longleftrightarrow> (\<exists>\<tau>. term_welltyped t \<tau> \<and> term_welltyped t' \<tau>)"
@@ -27,14 +21,8 @@ lemma atom_is_welltyped_iff [simp]:
   by simp
 
 sublocale literal: typing_lifting where
-  sub_typed = atom.typed and sub_welltyped = atom.welltyped and to_set = set_literal
+  sub_welltyped = atom.welltyped and to_set = set_literal
   by unfold_locales
-
-lemma literal_is_typed_iff [simp]:
-  "literal.is_typed (t \<approx> t') \<longleftrightarrow> atom.is_typed (Upair t t')"
-  "literal.is_typed (t !\<approx> t') \<longleftrightarrow> atom.is_typed (Upair t t')"
-  unfolding literal.is_typed_def
-  by simp_all
 
 lemma literal_is_welltyped_iff [simp]:
   "literal.is_welltyped (t \<approx> t') \<longleftrightarrow> atom.is_welltyped (Upair t t')"
@@ -42,17 +30,13 @@ lemma literal_is_welltyped_iff [simp]:
   unfolding literal.is_welltyped_def
   by simp_all
 
-lemma literal_is_typed_iff_atm_of: "literal.is_typed l \<longleftrightarrow> atom.is_typed (atm_of l)"
-  unfolding literal.is_typed_def
-  by (simp add: set_literal_atm_of)
-
 lemma literal_is_welltyped_iff_atm_of:
   "literal.is_welltyped l \<longleftrightarrow> atom.is_welltyped (atm_of l)"
   unfolding literal.is_welltyped_def
   by (simp add: set_literal_atm_of)
 
 sublocale clause: mulitset_typing_lifting where 
-  sub_typed = literal.typed and sub_welltyped = literal.welltyped
+  sub_welltyped = literal.welltyped
   by unfold_locales
 
 end
