thys/First_Order_Clause/Multiset_Typing_Lifting.thy
@@ -7,8 +7,8 @@ begin
 
 locale mulitset_typing_lifting = 
   typing_lifting where 
-  to_set = set_mset and sub_typed = sub_typed and sub_welltyped = sub_welltyped
-for sub_typed sub_welltyped :: "'sub \<Rightarrow> unit \<Rightarrow> bool"
+  to_set = set_mset and sub_welltyped = sub_welltyped
+  for sub_welltyped :: "'sub \<Rightarrow> unit \<Rightarrow> bool"
 begin
 
 sublocale natural_magma_with_empty_typing_lifting where
