thys/First_Order_Clause/Natural_Magma_Typing_Lifting.thy
@@ -4,22 +4,22 @@ theory Natural_Magma_Typing_Lifting
     Typing
 begin
 
-(* TODO: Generalize *)
 locale natural_magma_is_typed_lifting = 
   natural_magma where to_set = to_set +
-  typed_lifting where to_set = to_set and sub_typed = sub_typed
-  for to_set :: "'expr \<Rightarrow> 'sub set" and sub_typed :: "'sub \<Rightarrow> unit \<Rightarrow> bool"
+  typing_lifting where to_set = to_set and sub_welltyped = sub_welltyped
+  for to_set :: "'expr \<Rightarrow> 'sub set" and sub_welltyped :: "'sub \<Rightarrow> unit \<Rightarrow> bool"
 begin
 
-abbreviation (input) sub_is_typed where "sub_is_typed expr \<equiv> sub_typed expr ()"
+abbreviation (input) sub_is_welltyped where
+  "sub_is_welltyped expr \<equiv> sub_welltyped expr ()"
 
-lemma add [simp]: "is_typed (add sub M) \<longleftrightarrow> (sub_is_typed sub \<and> is_typed M)"
-  unfolding is_typed_def
+lemma add [simp]: "is_welltyped (add sub M) \<longleftrightarrow> (sub_is_welltyped sub \<and> is_welltyped M)"
+  unfolding is_welltyped_def
   by auto
 
 lemma plus [simp]:
-  "is_typed (plus M M') \<longleftrightarrow> is_typed M \<and> is_typed M'"
-  unfolding is_typed_def
+  "is_welltyped (plus M M') \<longleftrightarrow> is_welltyped M \<and> is_welltyped M'"
+  unfolding is_welltyped_def
   by auto
 
 end
@@ -28,21 +28,19 @@ locale natural_magma_with_empty_is_typed_lifting =
   natural_magma_is_typed_lifting + natural_magma_with_empty
 begin
 
-lemma empty [intro]: "is_typed empty"
-  unfolding is_typed_def
+lemma empty [intro]: "is_welltyped empty"
+  unfolding is_welltyped_def
   by simp
 
 end
 
 locale natural_magma_typing_lifting =
-  typed: natural_magma_is_typed_lifting where sub_typed = sub_typed  +
-  welltyped: natural_magma_is_typed_lifting where sub_typed = sub_welltyped +
+  welltyped: natural_magma_is_typed_lifting where sub_welltyped = sub_welltyped +
   typing_lifting +
   natural_magma
 
 locale natural_magma_with_empty_typing_lifting =
   natural_magma_typing_lifting + 
-  typed: natural_magma_with_empty_is_typed_lifting where sub_typed = sub_typed + 
-  welltyped: natural_magma_with_empty_is_typed_lifting where sub_typed = sub_welltyped
+  welltyped: natural_magma_with_empty_is_typed_lifting where sub_welltyped = sub_welltyped
 
 end
