thys/First_Order_Clause/Typed_Functional_Substitution_Lifting.thy
@@ -10,19 +10,19 @@ lemma ext_equiv: "(\<And>x. f x \<equiv> g x) \<Longrightarrow> f \<equiv> g"
 
 locale typed_functional_substitution_lifting =
   sub: typed_functional_substitution where
-  vars = sub_vars and subst = sub_subst and typed = sub_typed and base_vars = base_vars +
-  based_functional_substitution_lifting where to_set = to_set and base_vars = base_vars
+    vars = sub_vars and subst = sub_subst and welltyped = sub_welltyped and base_vars = base_vars +
+    based_functional_substitution_lifting where to_set = to_set and base_vars = base_vars
 for
-  sub_typed :: "('v, 'ty) var_types \<Rightarrow> 'sub \<Rightarrow> 'ty' \<Rightarrow> bool" and
+  sub_welltyped :: "('v, 'ty) var_types \<Rightarrow> 'sub \<Rightarrow> 'ty' \<Rightarrow> bool" and
   to_set :: "'expr \<Rightarrow> 'sub set" and
   base_vars :: "'base \<Rightarrow> 'v set"
 begin
 
-sublocale typed_lifting where sub_typed = "sub_typed \<V>"
+sublocale typing_lifting where sub_welltyped = "sub_welltyped \<V>"
   by unfold_locales
 
 sublocale typed_functional_substitution where
-  vars = vars and subst = subst and typed = typed
+  vars = vars and subst = subst and welltyped = welltyped
   by unfold_locales
 
 end
@@ -34,7 +34,7 @@ locale typed_grounding_functional_substitution_lifting =
 begin
 
 sublocale typed_grounding_functional_substitution where
-  vars = vars and subst = subst and typed = typed and to_ground = to_ground and
+  vars = vars and subst = subst and welltyped = welltyped and to_ground = to_ground and
   from_ground = from_ground
   by unfold_locales
 
@@ -44,47 +44,48 @@ end
 locale inhabited_typed_functional_substitution_lifting =
   typed_functional_substitution_lifting +
   sub: inhabited_typed_functional_substitution where
-  vars = sub_vars and subst = sub_subst and typed = sub_typed
+  vars = sub_vars and subst = sub_subst and welltyped = sub_welltyped
 begin
 
 sublocale inhabited_typed_functional_substitution where
-  vars = vars and subst = subst and typed = typed
+  vars = vars and subst = subst and welltyped = welltyped
   by unfold_locales (simp add: sub.types_inhabited)
 
 end
 
 locale typed_subst_stability_lifting =
   typed_functional_substitution_lifting +
-  sub: typed_subst_stability where typed = sub_typed and vars = sub_vars and subst = sub_subst
+  sub: typed_subst_stability where
+    welltyped = sub_welltyped and vars = sub_vars and subst = sub_subst
 begin
 
-sublocale typed_subst_stability where typed = typed and subst = subst and vars = vars
-  by unfold_locales (auto simp add: vars_def to_set_image is_typed_def)
+sublocale typed_subst_stability where welltyped = welltyped and subst = subst and vars = vars
+  by unfold_locales (auto simp add: vars_def to_set_image is_welltyped_def)
 
 end
 
 locale replaceable_\<V>_lifting =
   typed_functional_substitution_lifting +
-  sub: replaceable_\<V> where typed = sub_typed and vars = sub_vars and subst = sub_subst
+  sub: replaceable_\<V> where welltyped = sub_welltyped and vars = sub_vars and subst = sub_subst
 begin
 
 sublocale replaceable_\<V> where
-  subst = subst and vars = vars and typed = typed
-  by unfold_locales (metis SUP_upper2 sub.replace_\<V> subset_eq vars_def is_typed_def)
+  subst = subst and vars = vars and welltyped = welltyped
+  by unfold_locales (metis SUP_upper2 sub.replace_\<V> subset_eq vars_def is_welltyped_def)
 
 end
 
 locale typed_renaming_lifting =
   typed_functional_substitution_lifting where
-  base_typed = "base_typed :: ('v \<Rightarrow> 'ty) \<Rightarrow> 'base \<Rightarrow> 'ty \<Rightarrow> bool" +
+    base_welltyped = "base_welltyped :: ('v \<Rightarrow> 'ty) \<Rightarrow> 'base \<Rightarrow> 'ty \<Rightarrow> bool" +
   renaming_variables_lifting +
   sub: based_typed_renaming where
-  subst = sub_subst and vars = sub_vars and typed = sub_typed
+    subst = sub_subst and vars = sub_vars and welltyped = sub_welltyped
 begin
 
 sublocale based_typed_renaming where
-  subst = subst and vars = vars and typed = typed
-  by unfold_locales (force simp: vars_def subst_def is_typed_def)
+  subst = subst and vars = vars and welltyped = welltyped
+  by unfold_locales (force simp: vars_def subst_def is_welltyped_def)
 
 end
 
