thys/Superposition_Calculus/Superposition.thy
@@ -82,7 +82,7 @@ if
   "\<forall>x \<in> clause.vars D. \<V>\<^sub>2 x = \<V>\<^sub>3 (term.rename \<rho>\<^sub>2 x)"
   "is_welltyped_on (clause.vars E) \<V>\<^sub>1 \<rho>\<^sub>1"
   "is_welltyped_on (clause.vars D) \<V>\<^sub>2 \<rho>\<^sub>2"
-  "\<And>\<tau> \<tau>'. typed \<V>\<^sub>2 t\<^sub>2 \<tau> \<Longrightarrow> typed \<V>\<^sub>2 t\<^sub>2' \<tau>' \<Longrightarrow> \<tau> = \<tau>'"
+  "\<And>\<tau> \<tau>'. welltyped \<V>\<^sub>2 t\<^sub>2 \<tau> \<Longrightarrow> welltyped \<V>\<^sub>2 t\<^sub>2' \<tau>' \<Longrightarrow> \<tau> = \<tau>'"
 
 abbreviation eq_factoring_inferences where
   "eq_factoring_inferences \<equiv> { Infer [D] C | D C. eq_factoring D C }"
@@ -121,7 +121,7 @@ where
     \<forall>x \<in> clause.vars D. \<V>\<^sub>2 x = \<V>\<^sub>3 (term.rename \<rho>\<^sub>2 x) \<Longrightarrow>
     is_welltyped_on (clause.vars E) \<V>\<^sub>1 \<rho>\<^sub>1 \<Longrightarrow>
     is_welltyped_on (clause.vars D) \<V>\<^sub>2 \<rho>\<^sub>2 \<Longrightarrow>
-    (\<And>\<tau> \<tau>'. typed \<V>\<^sub>2 t\<^sub>2 \<tau> \<Longrightarrow> typed \<V>\<^sub>2 t\<^sub>2' \<tau>' \<Longrightarrow> \<tau> = \<tau>') \<Longrightarrow>
+    (\<And>\<tau> \<tau>'. welltyped \<V>\<^sub>2 t\<^sub>2 \<tau> \<Longrightarrow> welltyped \<V>\<^sub>2 t\<^sub>2' \<tau>' \<Longrightarrow> \<tau> = \<tau>') \<Longrightarrow>
     \<not> (E \<cdot> \<rho>\<^sub>1 \<odot> \<mu> \<preceq>\<^sub>c D \<cdot> \<rho>\<^sub>2 \<odot> \<mu>) \<Longrightarrow>
     (\<P> = Pos \<and> select E = {#} \<and> is_strictly_maximal (l\<^sub>1 \<cdot>l \<rho>\<^sub>1 \<odot> \<mu>) (E \<cdot> \<rho>\<^sub>1 \<odot> \<mu>) \<or>
      \<P> = Neg \<and> (select E = {#} \<and> is_maximal (l\<^sub>1 \<cdot>l \<rho>\<^sub>1 \<odot> \<mu>) (E \<cdot> \<rho>\<^sub>1 \<odot> \<mu>) \<or>
@@ -192,7 +192,7 @@ where
     \<forall>x \<in> clause.vars D. \<V>\<^sub>2 x = \<V>\<^sub>3 (term.rename \<rho>\<^sub>2 x) \<Longrightarrow>
     is_welltyped_on (clause.vars E) \<V>\<^sub>1 \<rho>\<^sub>1 \<Longrightarrow>
     is_welltyped_on (clause.vars D) \<V>\<^sub>2 \<rho>\<^sub>2 \<Longrightarrow>
-    (\<And>\<tau> \<tau>'. typed \<V>\<^sub>2 t\<^sub>2 \<tau> \<Longrightarrow> typed \<V>\<^sub>2 t\<^sub>2' \<tau>' \<Longrightarrow> \<tau> = \<tau>') \<Longrightarrow>
+    (\<And>\<tau> \<tau>'. welltyped \<V>\<^sub>2 t\<^sub>2 \<tau> \<Longrightarrow> welltyped \<V>\<^sub>2 t\<^sub>2' \<tau>' \<Longrightarrow> \<tau> = \<tau>') \<Longrightarrow>
     \<not> (E \<cdot> \<rho>\<^sub>1 \<odot> \<mu> \<preceq>\<^sub>c D \<cdot> \<rho>\<^sub>2 \<odot> \<mu>) \<Longrightarrow>
     select E = {#} \<Longrightarrow>
     is_strictly_maximal (l\<^sub>1 \<cdot>l \<rho>\<^sub>1 \<odot> \<mu>) (E \<cdot> \<rho>\<^sub>1 \<odot> \<mu>) \<Longrightarrow>
@@ -233,7 +233,7 @@ where
     \<forall>x \<in> clause.vars D. \<V>\<^sub>2 x = \<V>\<^sub>3 (term.rename \<rho>\<^sub>2 x) \<Longrightarrow>
     is_welltyped_on (clause.vars E) \<V>\<^sub>1 \<rho>\<^sub>1 \<Longrightarrow>
     is_welltyped_on (clause.vars D) \<V>\<^sub>2 \<rho>\<^sub>2 \<Longrightarrow>
-    (\<And>\<tau> \<tau>'. typed \<V>\<^sub>2 t\<^sub>2 \<tau> \<Longrightarrow> typed \<V>\<^sub>2 t\<^sub>2' \<tau>' \<Longrightarrow> \<tau> = \<tau>') \<Longrightarrow>
+    (\<And>\<tau> \<tau>'. welltyped \<V>\<^sub>2 t\<^sub>2 \<tau> \<Longrightarrow> welltyped \<V>\<^sub>2 t\<^sub>2' \<tau>' \<Longrightarrow> \<tau> = \<tau>') \<Longrightarrow>
     \<not> (E \<cdot> \<rho>\<^sub>1 \<odot> \<mu> \<preceq>\<^sub>c D \<cdot> \<rho>\<^sub>2 \<odot> \<mu>) \<Longrightarrow>
     (select E = {#} \<Longrightarrow> is_maximal (l\<^sub>1 \<cdot>l \<rho>\<^sub>1 \<odot> \<mu>) (E \<cdot> \<rho>\<^sub>1 \<odot> \<mu>)) \<Longrightarrow>
     (select E \<noteq> {#} \<Longrightarrow> is_maximal (l\<^sub>1 \<cdot>l \<rho>\<^sub>1 \<odot> \<mu>) ((select E) \<cdot> \<rho>\<^sub>1 \<odot> \<mu>)) \<Longrightarrow>
